fix definition of query and do the Betree -> map refinement for query

disk-betree/BetreeSpec.dfy
@@ -60,8 +60,24 @@ module BetreeSpec {
 
   datatype LookupQuery = LookupQuery(key: Key, value: Value, lookup: Lookup)
 
+  predicate ValidLayerIndex(lookup: Lookup, idx: int) {
+    && 0 <= idx < |lookup|
+  }
+
   predicate LookupVisitsWFNodes(lookup: Lookup) {
     forall i :: 0 <= i < |lookup| ==> WFNode(lookup[i].node)
+  }
+
+  predicate LookupFollowsChildRefAtLayer(key: Key, lookup: Lookup, idx: int)
+  requires ValidLayerIndex(lookup, idx) && idx < |lookup| - 1;
+  requires key in lookup[idx].node.children;
+  {
+    lookup[idx].node.children[key] == lookup[idx+1].ref
+  }
+
+  predicate LookupFollowsChildRefs(key: Key, lookup: Lookup) {
+    && (forall idx :: ValidLayerIndex(lookup, idx) && idx < |lookup| - 1 ==> key in lookup[idx].node.children)
+    && (forall idx :: ValidLayerIndex(lookup, idx) && idx < |lookup| - 1 ==> LookupFollowsChildRefAtLayer(key, lookup, idx))
   }
 
   function InterpretLookup(lookup: Lookup, key: Key) : G.M.Message
@@ -71,6 +87,9 @@ module BetreeSpec {
   }
 
   predicate ValidQuery(q: LookupQuery) {
+    && |q.lookup| > 0
+    && q.lookup[0].ref == Root()
+    && LookupFollowsChildRefs(q.key, q.lookup)
     && LookupVisitsWFNodes(q.lookup)
     && BufferDefinesValue(InterpretLookup(q.lookup, q.key), q.value)
   }
